lnt_contraction_mr.v
@@ -1,0 +1,1030 @@
+Require Import ssreflect.
+ 
+Require Import gen.
+Require Import dd.
+Require Import List_lemmas.
+Require Import lnt lntacs lntls lntbR lntmtacs.
+Require Import lntb1L lntb2L.
+Require Import lnt_weakening.
+Require Import lntkt_exch.
+Require Import swapped.
+Require Import lnt_contraction.
+
+(* ------- *)
+(* TACTICS *)
+(* ------- *)
+
+Ltac ms_cgs_cont acm := 
+rewrite dersrec_map_single ;
+rewrite -> Forall_map_single in acm ;
+rewrite -> ?can_gen_contL_gen_def' in acm ;
+rewrite -> ?can_gen_contR_gen_def' in acm ;
+unfold nslclext ; unfold nslext.
+
+Ltac use_acm_os_cont acm rs swap ith :=
+(* swap in opposite side from where rule active *)
+derIrs rs ; [> 
+apply NSlclctxt || apply NSlctxt ;
+apply ith |
+ms_cgs_cont acm ;
+eapply acm in swap ] ;
+[> eapply swap |
+  unfold nslext ; unfold nslclext ; reflexivity |
+  reflexivity ].
+
+Ltac nsgen_sw_cont rs sppc c c' acm inps0 swap :=
+derIrs rs ; [>
+  (assoc_mid c ; apply NSlctxt') ||
+  (assoc_single_mid' c ; apply NSctxt') ||
+  (list_assoc_l' ; apply NSlclctxt') ||
+  (list_assoc_l' ; apply NSlcctxt') ;
+  exact sppc |
+rewrite dersrec_forall ;
+intros q qin ;
+rewrite -> in_map_iff in qin ; cE ; subst q ;
+rewrite -> Forall_forall in acm ;
+rename_last inps0 ;  eapply in_map in inps0 ;
+eapply acm in inps0 ;
+rewrite -> ?can_gen_contL_gen_def' in inps0 ;
+rewrite -> ?can_gen_contR_gen_def' in inps0 ; 
+unfold nsext ; unfold nslext ;  unfold nslcext ; unfold nslclext ;
+assoc_single_mid' c' ;
+eapply inps0 ; [> exact swap |
+  unfold nsext ; unfold nslext ;  unfold nslcext ; unfold nslclext ;
+  list_eq_assoc | reflexivity ]].
+
+Ltac rem_nil_hyp :=
+  repeat match goal with
+  | [ H : context[ [] ++ ?A ] |- _ ] => rem_nil_hyp_arg H
+  | [ H : context[ ?A ++ [] ] |- _ ] => rem_nil_hyp_arg H
+  | _ => idtac
+  end.
+
+Ltac rem_nil := rem_nil_hyp; rem_nil_goal.
+
+Ltac check_nil_cons_contr :=
+  match goal with
+  | [H : [] = ?l1 ++ ?a :: ?l2 |- _] => contradiction (nil_eq_list l1 l2 a H)
+  | [H : ?l1 ++ ?a :: ?l2 = [] |- _] => symmetry in H; contradiction (nil_eq_list l1 l2 a H)
+  | _ => idtac
+  end.
+
+Ltac cont_solve2 :=
+   match goal with
+   | [ |- context[?a :: ?l]] =>
+     match l with
+     | context[?a :: ?l2] =>  
+   list_assoc_r_single;
+   eapply (contracted_gen__spec a);
+   cont_solve
+     end
+   end.
+
+Ltac cont_setup_constr constr :=
+  match goal with
+  | [ |- context[ (@constr ?V ?A) :: ?l ] ] => list_assoc_r_single; assoc_mid ([@constr V A])
+  end.
+
+Ltac use_acm1_cont_constr acm rs ith constr :=
+     derIrs rs; [ 
+apply NSlctxt2 || apply NSlclctxt' ;
+cont_setup_constr constr;
+apply ith | 
+ms_cgs_cont acm ;
+  list_assoc_r' ; simpl] ;
+   first [eapply acm | list_assoc_l'; rewrite <- app_assoc; eapply acm];
+   unfold nslext ; unfold nslclext ; list_assoc_r' ; simpl; try reflexivity; cont_solve2.
+
+Ltac use_acm2s_cont acm rs ith :=
+derIrs rs ; [> 
+list_assoc_r' ; simpl ; apply NSlctxt2 || apply NSlclctxt' ;
+apply ith |
+ms_cgs_cont acm ;
+list_assoc_r' ; simpl ;
+rewrite ?list_rearr22 ; eapply acm ] ; [> | 
+  unfold nslext ; unfold nslclext ; list_assoc_r' ; simpl ; reflexivity |
+  reflexivity ] ; cont_solve2.
+
+Ltac cont_setup_apply_constr constr :=
+  list_assoc_r_single;
+  match goal with
+  | [ acm : context[ @constr ?V ?A ] |- _ ] =>
+    repeat match goal with
+    | [ acm : context[ ?l1 ++ A :: ?l2 ++ ?l3 ] |-
+        derrec ?rules ?p (?G1 ++ ?G2 ++ [(?K1,?K2,?d)]) ] =>
+      match K1 with
+      | ?l5 ++ l2 ++ ?l4 => idtac
+      | ?l5 ++ ?l4 => rewrite (app_assoc l5)
+      end
+    end
+  end.
+
+Ltac cont_setup_apply_constr2 constr :=
+  list_assoc_r_single;
+  match goal with
+  | [ acm : context[ @constr ?V ?A ] |- _ ] =>
+    repeat match goal with
+    | [ acm : context[ ?l1 ++ A :: ?l2 ++ ?l3 ] |-
+        derrec ?rules ?p (?G1 ++ ?G2 ++ [(?K1,?K2,?d)]) ] =>
+      match K1 with
+      | ?l5 ++ l3 ++ ?l4 => idtac
+      | ?l5 ++ ?l4 => rewrite (app_assoc l5)
+      end
+    end
+  end.
+
+Ltac cont_setup_apply_constr3 constr :=
+  list_assoc_r_single;
+  match goal with
+  | [ acm : context[ @constr ?V ?A ] |- _ ] =>
+    repeat match goal with
+    | [ acm : context[ ?l1 ++ A :: ?l2 ] |-
+        derrec ?rules ?p (?G1 ++ ?G2 ++ [(?K1,?K2,?d)]) ] =>
+      match K1 with
+      | ?l5 ++ l2 ++ ?l4 => idtac
+      | ?l5 ++ ?l4 => rewrite (app_assoc l5)
+      end
+    end
+  end.
+
+Ltac use_acm2s_cont' acm rs ith constr :=
+  derIrs rs ;
+  [> apply NSlctxt2 || apply NSlclctxt' ;
+   apply ith |
+   ms_cgs_cont acm ;
+   list_assoc_r' ; simpl ;
+   rewrite ?list_rearr22 ; eapply acm ] ;
+  [> | unfold nslext ; unfold nslclext ; list_assoc_r' ; simpl ; reflexivity |
+  reflexivity ] ; cont_solve2.
+
+Ltac use_acm_sw_sep_cont acm rs weak ith :=
+(* interchange two sublists of list of formulae,
+  no need to expand swap (swap separate from where rule is applied) *)
+derIrs rs ; [> 
+list_assoc_r' ; simpl ; apply NSlclctxt' || apply NSlctxt2 ;
+apply ith |
+ms_cgs_cont acm ;
+eapply acm in weak ] ;
+[> (rewrite - list_rearr21 ; eapply weak) || 
+  (list_assoc_r' ; simpl ; eapply weak) |
+  unfold nslext ; unfold nslclext ; list_assoc_r' ; simpl ; reflexivity |
+  reflexivity ].
+
+Ltac cont_setup_apply_constr4 constr :=
+  list_assoc_r_single;
+  repeat match goal with
+         | [ acm : context[ ?l1 ++ @constr ?V ?A :: ?l2 ++ ?l3 ] |-
+             derrec ?rules ?p (?G1 ++ [(?K1,?K2,?d)] ++ ?G2) ] =>
+           match K1 with
+           | ?l5 ++ l2 ++ ?l4 => idtac 
+           | ?l5 ++ ?l4 => rewrite (app_assoc l5)
+           end
+         end.
+
+Ltac cont_setup_apply_constr5 constr :=
+  list_assoc_r_single;
+  repeat match goal with
+         | [ acm : context[ ?l1 ++ @constr ?V ?A :: ?l3 ++ ?l2 ] |-
+             derrec ?rules ?p (?G1 ++ [(?K1,?K2,?d)] ++ ?G2) ] =>
+           match K1 with
+           | ?l5 ++ l2 ++ ?l4 => idtac 
+           | ?l5 ++ ?l4 => rewrite (app_assoc l5)
+           end
+         end.
+
+Ltac cont_setup_apply_constr6 constr :=
+  list_assoc_r_single;
+  repeat match goal with
+         | [ acm : context[ ?l1 ++ @constr ?V ?A :: ?l2 ] |-
+             derrec ?rules ?p (?G1 ++ [(?K1,?K2,?d)] ++ ?G2) ] =>
+           match K1 with
+           | ?l5 ++ l2 ++ ?l4 => idtac 
+           | ?l5 ++ ?l4 => rewrite (app_assoc l5)
+           end
+         end.
+
+Ltac cont_setup_apply_constr7 constr:=
+  list_assoc_r_single;
+  repeat match goal with
+         | [ acm : context[ ?l1 ++ @constr ?V ?A :: ?l2 ] |-
+             derrec ?rules ?p (?G1 ++ ?G2 ++ [(?K1,?K2,?d)]) ] =>
+           match K1 with
+           | ?l5 ++ [@constr V A] ++ ?l4 => idtac 
+           | ?l5 ++ ?l4 => rewrite (app_assoc l5)
+           end
+         end.
+
+Ltac no_use_acm_cont rs drs constr:=
+  derIrs rs;
+  [apply NSlclctxt'; apply constr |
+   exact drs].
+
+Ltac acmi_snr_cont acmi swap := 
+  eapply acmi ; [> apply nslclext_def | reflexivity ].
+
+Ltac use_acm_2_cont acm rs swap ith :=
+derIrs rs ; [>
+apply NSlclctxt' || apply NSlctxt2 ;
+apply ith |
+ms_cgs acm ; destruct acm as [acm1 acm2] ; 
+inversion swap; (subst; split ; 
+[ acmi_snr_cont acm1 swap | acmi_snr_cont acm2 swap ])
+            ].
+
+Lemma can_gen_contL_gen_imp: forall {V : Set} 
+  (rules : rls (list (rel (list (PropF V)) * dir))) ns,
+  can_gen_contL_gen rules ns -> forall G K seq Γ Δ Γ' (d : dir), 
+  contracted_gen Γ Γ' -> ns = G ++ (seq, d) :: K -> seq = pair Γ Δ ->
+    derrec rules (fun _ => False) (G ++ (pair Γ' Δ, d) :: K).
+Proof.  intros until 0. intro.
+  rewrite -> can_gen_contL_gen_def' in H. exact H. Qed.
+
+Lemma can_gen_contR_gen_imp: forall {V : Set} 
+  (rules : rls (list (rel (list (PropF V)) * dir))) ns,
+  can_gen_contR_gen rules ns -> forall G K seq Γ Δ Δ' (d : dir), 
+  contracted_gen Δ Δ' -> ns = G ++ (seq, d) :: K -> seq = pair Γ Δ ->
+    derrec rules (fun _ => False) (G ++ (pair Γ Δ', d) :: K).
+Proof.  intros until 0. intro.
+  rewrite -> can_gen_contR_gen_def' in H. exact H. Qed.
+
+
+Ltac contL2 rs sppc acm swap :=
+derIrs rs ; [> list_assoc_l' ;
+    apply NSlclctxt' || apply NSlctxt2 ; exact sppc | ] ;
+rewrite dersrec_forall ; intros L H ;
+rewrite -> in_map_iff in H ; destruct H ; destruct H as [H1 H2] ; subst ;
+rewrite -> Forall_forall in acm ; eapply in_map in H2 ; eapply acm in H2 ;
+eapply can_gen_contL_gen_imp in H2 || eapply can_gen_contR_gen_imp in H2 ;
+  [> | exact swap | | reflexivity ] ;
+  [> unfold nslclext ; list_assoc_r' ; exact H2
+    | unfold nslclext ; list_assoc_r' ; reflexivity].
+
+Ltac use_acm_2_snd_cont acm rs swap ith :=
+derIrs rs ; [ list_assoc_r' ;
+apply NSlclctxt' || apply NSlctxt2 ;
+apply ith |
+ms_cgs acm ; destruct acm as [acm1 acm2] ; 
+inversion swap; (subst; split;
+[ acmi_snr_snd_weak acm1 swap | acmi_snr_snd_weak acm2 swap ])
+            ].
+
+
+Ltac ltstart' acm acm1 acm2 :=
+  ms_cgs acm ; destruct acm as [acm1 acm2];
+  list_assoc_r_s_arg acm1;
+  list_assoc_r_s_arg acm2;
+  list_assoc_r_single.
+
+Ltac ltsolve' acm1a acm1b acm2a acm2b :=
+  list_assoc_r_s_arg acm1a;
+  list_assoc_r_s_arg acm1b;
+  list_assoc_r_s_arg acm2a;
+  list_assoc_r_s_arg acm2b;
+  list_assoc_r_single;
+  split; [ exact acm1a || exact acm1b | exact acm2a || exact acm2b].
+
+Ltac ltsolve_pre acm1a acm1b acm2a acm2b :=
+  list_assoc_r_s_arg acm1a;
+  list_assoc_r_s_arg acm1b;
+  list_assoc_r_s_arg acm2a;
+  list_assoc_r_s_arg acm2b;
+  list_assoc_r_single.
+
+Ltac ltsolve_end acm1a acm1b acm2a acm2b :=
+    split; [ exact acm1a || exact acm1b | exact acm2a || exact acm2b].
+
+Ltac ltmidacm' acm1 acm2 acm1a acm1b acm2a acm2b :=
+  edestruct acm1 as [acm1a acm1b]; [reflexivity | reflexivity |];
+  edestruct acm2 as [acm2a acm2b]; [reflexivity | reflexivity |].
+
+
+Ltac ltbrack1 acm1 a :=
+  repeat match type of acm1 with
+  | can_gen_contR_gen ?rules (nslclext ?G ([(?Γ, ?l, ?d)] ++ ?seq)) =>
+    match l with
+    | [a] ++ ?l2 => idtac
+    | ?l2 ++ [a] ++ ?l3 => idtac
+    | ?l2 ++ (?l3 ++ ?l4) => rewrite (app_assoc l2) in acm1
+    end
+         end.
+
+Ltac ltbrack2 acm1 a :=
+  repeat match type of acm1 with
+  | can_gen_contR_gen ?rules (nslclext ?G ([(?Γ, ?l, ?d)] ++ ?seq)) =>
+    match l with
+    | [a] ++ ?l2 => idtac
+    | ?l2 ++ [a] ++ ?l3 ++ [a] ++ ?l4 => idtac
+    | ?l2 ++ [a] ++ ?l3 ++ ?l4 => rewrite (app_assoc l3) in acm1
+    end
+         end.
+
+Ltac assoc_mid_hyp l H := 
+  list_assoc_r_s_arg H ;
+  rewrite ?app_comm_cons in H ;
+  repeat ((rewrite - (app_assoc _ l _) in H; fail 1) || rewrite app_assoc in H) ;
+  rewrite - (app_assoc _ l _)  in H.
+
+Ltac ltbrack_concl_pre Γ l :=
+  repeat match goal with
+  | [ |- context[ (Γ, ?l1, ?d) ] ] =>
+    match l1 with
+    | l ++ ?l2 => idtac
+    | ?l2 ++ ?l3 => rewrite (app_assoc l2)
+    end
+         end.
+
+Ltac ltbrack_concl acm1 :=
+  match type of acm1 with
+  | context[ [(?Γ, ?l1 ++ [?A] ++ ?l2, ?d)] ++ ?seq ] =>
+    ltbrack_concl_pre Γ l1
+  end.
+
+Ltac ltapplyrule rs WBox1Rs acm1 :=
+  derIrs rs; [apply NSlclctxt'; simpl; apply WBox1Rs |
+              list_assoc_r_single; ms_cgs acm1].
+
+Ltac ltsolve_full_pre acm acm1 acm2 acm1a acm1b acm2a acm2b A rs WBox1Rs a :=
+  ltstart' acm acm1 acm2;
+  assoc_mid_hyp [A] acm1;
+  ltbrack_concl acm1;
+  ltapplyrule rs WBox1Rs acm1;
+  list_assoc_r_s_arg acm1;
+  list_assoc_r_s_arg acm2;
+  ltbrack1 acm1 a;
+  ltbrack2 acm1 a;
+  ltbrack1 acm2 a;
+  ltbrack2 acm2 a;
+  ltmidacm' acm1 acm2 acm1a acm1b acm2a acm2b.
+
+Ltac apply_exch Hexch :=
+  eapply Hexch; [tauto | | reflexivity | reflexivity].
+
+Ltac sep_nil :=
+  match goal with
+  | [ |- context[ [?a] ++ [?a] ++ ?l2] ] =>
+    rewrite <- (app_nil_l ([a] ++ l2))
+  end.
+
+Ltac ltapplyrule2 rs rw WBox1Rs acm1 :=
+  derIrs rs; [apply NSlclctxt'; rw; simpl; apply WBox1Rs |
+  list_assoc_r_single; ms_cgs acm1].
+
+Ltac ltbrack1_snd acm1 a :=
+  repeat match type of acm1 with
+  | can_gen_contR_gen ?rules (nslclext ?G (?seq ++ [(?Γ, ?l, ?d)])) =>
+    match l with
+    | [a] ++ ?l2 => idtac
+    | ?l2 ++ [a] ++ ?l3 => idtac
+    | ?l2 ++ (?l3 ++ ?l4) => rewrite (app_assoc l2) in acm1
+    end
+  end.
+
+Ltac ltbrack2_snd acm1 a :=
+  repeat match type of acm1 with
+  | can_gen_contR_gen ?rules (nslclext ?G (?seq ++ [(?Γ, ?l, ?d)])) =>
+    match l with
+    | [a] ++ ?l2 => idtac
+    | ?l2 ++ [a] ++ ?l3 ++ [a] ++ ?l4 => idtac
+    | ?l2 ++ [a] ++ ?l3 ++ ?l4 => rewrite (app_assoc l3) in acm1
+    end
+  end.
+
+Ltac ltbrack1_mid acm1 a :=
+  repeat match type of acm1 with
+  | can_gen_contR_gen ?rules (nslclext ?G (?seq ++ [(?Γ, ?l, ?d)] ++ ?seq2)) =>
+    match l with
+    | [a] ++ ?l2 => idtac
+    | ?l2 ++ [a] ++ ?l3 => idtac
+    | ?l2 ++ (?l3 ++ ?l4) => rewrite (app_assoc l2) in acm1
+    end
+  end.
+
+Ltac ltbrack2_mid acm1 a :=
+  repeat match type of acm1 with
+  | can_gen_contR_gen ?rules (nslclext ?G (?seq ++ [(?Γ, ?l, ?d)] ++ ?seq2)) =>
+    match l with
+    | [a] ++ ?l2 => idtac
+    | ?l2 ++ [a] ++ ?l3 ++ [a] ++ ?l4 => idtac
+    | ?l2 ++ [a] ++ ?l3 ++ ?l4 => rewrite (app_assoc l3) in acm1
+    end
+  end.
+
+Ltac ltmidacm'2 acm1 acm2 acm1a acm1b acm2a acm2b G :=
+  edestruct acm1 as [acm1a acm1b];
+  [unfold nslclext; rewrite (app_assoc G); reflexivity | reflexivity |];
+  edestruct acm2 as [acm2a acm2b];
+  [unfold nslclext; rewrite (app_assoc G); reflexivity | reflexivity |].  
+
+Ltac ltsolve_full_pre2 acm acm1 acm2 acm1a acm1b acm2a acm2b A rs Constr WBox1Rs a G:=
+  ltstart' acm acm1 acm2;
+  assoc_mid_hyp [A] acm1;
+  ltbrack_concl acm1;
+  ltapplyrule2 rs ltac : (assoc_mid [(@Constr _  A)]) WBox1Rs acm1;
+  list_assoc_r_s_arg acm1;
+  list_assoc_r_s_arg acm2;
+  ltbrack1_snd acm1 a;
+  ltbrack2_snd acm1 a;
+  ltbrack1_mid acm2 a;
+  ltbrack2_mid acm2 a;
+  ltmidacm'2 acm1 acm2 acm1a acm1b acm2a acm2b G.
+
+Ltac ltmidacm'3 acm1 acm2 acm1a acm1b acm2a acm2b G :=
+  edestruct acm1 as [acm1a acm1b];
+  [unfold nslclext; rewrite (app_assoc G); reflexivity | try sep_nil; reflexivity |];
+  edestruct acm2 as [acm2a acm2b];
+  [unfold nslclext; rewrite (app_assoc G); reflexivity | try sep_nil ; reflexivity |].
+
+Ltac ltsolve_full_pre3 acm acm1 acm2 acm1a acm1b acm2a acm2b A rs Constr WBox1Rs a G:=
+  ltstart' acm acm1 acm2;
+  ltbrack_concl acm1;
+  ltapplyrule2 rs ltac : (assoc_mid [@Constr _ A]) WBox1Rs acm1;
+  list_assoc_r_s_arg acm1;
+  list_assoc_r_s_arg acm2;
+  ltbrack1_snd acm1 a;
+  ltbrack2_snd acm1 a;
+  ltbrack1_mid acm2 a;
+  ltbrack2_mid acm2 a;
+  list_assoc_r_s_arg acm1;
+  list_assoc_r_s_arg acm2;
+  ltmidacm'3 acm1 acm2 acm1a acm1b acm2a acm2b G.
+
+Ltac b1R_extra1 Hexch acm1b acm2a A0 :=
+  split;
+  [rewrite (app_assoc A0); apply_exch Hexch;
+   list_assoc_r_single; apply_exch Hexch;
+   exact acm1b |
+   apply_exch Hexch; exact acm2a].
+
+Ltac b1R_extra2 Hexch acm1b acm2b A0 H4 :=
+  split;
+  [rewrite (app_assoc A0); rewrite (app_assoc H4);
+   apply_exch Hexch; list_assoc_r_single; exact acm1b |
+   exact acm2b].
+
+Ltac b1R_extra3 Hexch acm1b acm2b A0 :=
+  split;
+  [rewrite (app_assoc A0); apply_exch Hexch;
+   list_assoc_r_single; exact acm1b | exact acm2b].
+
+Ltac b1R_extra1_look Hexch acm1b acm2a :=
+  match goal with
+  | [ |- context[ _ ++ [(?Γ, ?A0 ++ ?l, ?d)] ++ _ ] ] =>
+    b1R_extra1 Hexch acm1b acm2a A0
+  end.
+
+Ltac b1R_extra2_look Hexch acm1b acm2b :=
+  match goal with
+  | [ |- context[ _ ++ [(?Γ, ?A0 ++ ?l ++ ?H4 ++ ?l2, ?d)] ++ _ ] ] =>
+    b1R_extra2 Hexch acm1b acm2b A0 H4
+  end.
+
+Ltac b1R_extra3_look Hexch acm1b acm2b :=
+  match goal with
+  | [ |- context[ _ ++ [(?Γ, ?A0 ++ ?l, ?d)] ++ _ ] ] =>
+    b1R_extra3 Hexch acm1b acm2b A0
+  end.
+
+Ltac ltsolve_full acm A rs WBox1Rs a Hexch :=
+  let acm1 := fresh "acm1" in let acm2 := fresh "acm2" in
+  let acm1a := fresh "acm1a" in let acm1b := fresh "acm1b" in
+  let acm2a := fresh "acm2a" in let acm2b := fresh "acm2b" in               
+  ltsolve_full_pre acm acm1 acm2 acm1a acm1b acm2a acm2b A rs WBox1Rs a;
+  ltsolve_pre acm1a acm1b acm2a acm2b;
+  try ltsolve_end acm1a acm1b acm2a acm2b;   
+  b1R_extra1_look Hexch acm1b acm2a ||
+  b1R_extra2_look Hexch acm1b acm2b ||
+  b1R_extra3_look Hexch acm1b acm2b.
+
+Ltac ltsolve_full23 acm A rs WBox WBox1Rs a G :=
+  let acm1 := fresh "acm1" in let acm2 := fresh "acm2" in
+  let acm1a := fresh "acm1a" in let acm1b := fresh "acm1b" in
+  let acm2a := fresh "acm2a" in let acm2b := fresh "acm2b" in               
+  (ltsolve_full_pre2 acm acm1 acm2 acm1a acm1b acm2a acm2b A rs WBox WBox1Rs a G ||
+  ltsolve_full_pre3 acm acm1 acm2 acm1a acm1b acm2a acm2b A rs WBox WBox1Rs a G);
+  ltsolve' acm1a acm1b acm2a acm2b.
+   
+Ltac process swap :=
+  inversion_clear swap; subst;
+  repeat (acacDe ; subst ; simpl ; rem_nil).
+    
+
+(* ------------------------ *)
+(* CONTRACTION FOR B2RRULES *)
+(* ------------------------ *)
+
+Lemma gen_contL_gen_step_b2R_lc: forall V ps concl last_rule rules,
+  last_rule = nslclrule (@b2rrules V) ->
+  gen_contL_gen_step last_rule rules ps concl.
+Proof.  intros until 0.  unfold gen_contL_step.
+intros lreq nsr drs acm rs. clear drs. subst.
+
+inversion nsr as [? ? ? sppc mnsp nsc]. clear nsr.
+unfold nslclext in nsc.
+rewrite can_gen_contL_gen_def'.  intros until 0. intros weak pp ss.
+unfold nslclext in pp. subst.
+
+acacD' ; subst ; rewrite -> ?app_nil_r in *. (* 3 subgoals, the various locs
+  where the exchange might be relative to where the rule is active *)
+
+-{ inversion sppc ; subst ; clear sppc. (* 2 subgoals *)
+   + use_acm_os_cont acm rs weak WBox2Rs.
+   + use_acm_os_cont acm rs weak BBox2Rs. }
+(* case of exchange in sequent to the left of where rule applied *)
+-{ nsgen_sw_cont rs sppc c (Γ', Δ, d) acm inps0 weak. }
+-{ inversion sppc ; subst ; clear sppc. (* 2 subgoals *)
+  +{ acacDe ; subst ; simpl ; rewrite ?app_nil_r. (* 1 subgoals *)
+    * use_acm_os_cont acm rs weak WBox2Rs.
+    }
+  +{ acacDe ; subst ; simpl ; rewrite ?app_nil_r. (* 1 subgoals *)
+    * use_acm_os_cont acm rs weak BBox2Rs.
+    }
+  }
+Qed.
+
+Lemma gen_contR_gen_step_b2R_lc: forall V ps concl last_rule rules,
+  last_rule = nslclrule (@b2rrules V) ->
+  gen_contR_gen_step last_rule rules ps concl.
+Proof.  intros until 0.  unfold gen_swapR_step.
+intros lreq nsr drs acm rs. clear drs. subst.
+
+inversion nsr as [? ? ? sppc mnsp nsc]. clear nsr.
+unfold nslclext in nsc.
+rewrite can_gen_contR_gen_def'.  intros until 0. intros weak pp ss.
+unfold nslclext in pp. subst.
+
+acacD' ; subst ; rewrite -> ?app_nil_r in *. (* 3 subgoals, the various locs
+  where the exchange might be relative to where the rule is active *)
+
+-{ inversion sppc ; subst ; clear sppc. (* 2 subgoals *)
++{ inversion_clear weak; subst;
+   repeat (acacD' ; subst ; simpl ; rem_nil) ;
+   try discriminate; rem_nil; subst;
+   check_nil_cons_contr;   
+   use_acm1_cont_constr acm rs WBox2Rs WBox. }
++{ inversion_clear weak; subst;
+   repeat (acacD' ; subst ; simpl ; rem_nil) ;
+   try discriminate; rem_nil; subst;
+   check_nil_cons_contr;
+   use_acm1_cont_constr acm rs BBox2Rs BBox.
+     (* 10 subgoals *)
+}
+}
+-{ nsgen_sw_cont rs sppc c (Γ, Δ', d) acm inps0 weak. }
+-{ inversion sppc ; subst ; clear sppc.  (* 2 subgoals *)
+(* WBox *)
++{ acacDe ; subst ; simpl ; rewrite ?app_nil_r. (* 1 subgoals *)
+*{ inversion_clear weak; subst;
+   repeat (acacD' ; subst ; simpl ; rem_nil) ;
+   try discriminate; rem_nil; subst;
+   check_nil_cons_contr;   
+    use_acm1_cont_constr acm rs WBox2Rs WBox. }
+}
+(* BBox *)
++{ acacDe ; subst ; simpl ; rewrite ?app_nil_r. (* 1 subgoals *)
+*{ inversion_clear weak; subst;
+   repeat (acacD' ; subst ; simpl ; rem_nil) ;
+   try discriminate; rem_nil; subst;
+   check_nil_cons_contr;   
+    use_acm1_cont_constr acm rs BBox2Rs BBox. }
+} }
+Qed.
+
+
+(* ------------------------ *)
+(* CONTRACTION FOR B1LRULES *)
+(* ------------------------ *)
+
+Lemma gen_contL_gen_step_b1L_lc: forall V ps concl last_rule rules,
+  last_rule = nslclrule (@b1lrules V) ->
+  gen_contL_gen_step last_rule rules ps concl.
+Proof.  intros until 0.  unfold gen_weakL_step.
+intros lreq nsr drs acm rs. clear drs. subst.
+
+inversion nsr as [? ? ? sppc mnsp nsc]. clear nsr.
+unfold nslclext in nsc.
+rewrite can_gen_contL_gen_def'.  intros until 0. intros weak pp ss.
+unfold nslclext in pp. subst.
+
+acacD' ; subst ; rewrite -> ?app_nil_r in *. (* 3 subgoals, the various locs
+  where the exchange might be relative to where the rule is active *)
+
+(* swap in the first of the two sequents affected by the rule *)
+-{ inversion sppc ; subst ; clear sppc. (* 2 subgoals *)
+   +{ inversion_clear weak; subst;
+      repeat (acacD' ; subst ; simpl ; rem_nil) ;
+      try discriminate; rem_nil; subst;
+      check_nil_cons_contr;
+      use_acm1_cont_constr acm rs WBox1Ls WBox.
+    }
+   +{ inversion_clear weak; subst;
+      repeat (acacD' ; subst ; simpl ; rem_nil) ;
+      try discriminate; rem_nil; subst;
+      check_nil_cons_contr;
+      use_acm1_cont_constr acm rs BBox1Ls BBox.
+    }
+ }
+(* case of exchange in sequent to the left of where rule applied *)
+-{ nsgen_sw_cont rs sppc c (Γ', Δ, d) acm inps0 weak. }
+
+(* here, weak in either of the two sequents affected by the rule *)
+-{ inversion sppc ; subst ; clear sppc. (* 2 subgoals *)
+
+(* WBox *)
++{ acacDe ; subst ; simpl ; rewrite ?app_nil_r. (* 2 subgoals *)
+*{ inversion_clear weak; subst;
+      repeat (acacD' ; subst ; simpl ; rem_nil) ;
+      try discriminate; rem_nil; subst;
+      check_nil_cons_contr;
+      use_acm1_cont_constr acm rs WBox1Ls WBox.
+ }
+(* swapping in second sequent of principal rule *) 
+*{
+inversion_clear weak; subst;
+acacD' ; subst;
+  try (  acacDe; subst; rem_nil;
+  (cont_setup_apply_constr WBox;
+   use_acm2s_cont' acm rs WBox1Ls WBox) ||
+  (cont_setup_apply_constr2 WBox;
+   use_acm2s_cont' acm rs WBox1Ls WBox) ||
+  (cont_setup_apply_constr3 WBox;
+   use_acm2s_cont' acm rs WBox1Ls WBox)).
+(* 4 subgoals, cases of where swapping occurs in the two parts
+  of context in conclusion (where no principal formula) *)
+
+{ use_acm2s_cont acm rs WBox1Ls. }
+  }
+  }
+
+(* WBox *)
++{ acacDe ; subst ; simpl ; rewrite ?app_nil_r. (* 2 subgoals *)
+*{ inversion_clear weak; subst;
+      repeat (acacD' ; subst ; simpl ; rem_nil) ;
+      try discriminate; rem_nil; subst;
+      check_nil_cons_contr;
+      use_acm1_cont_constr acm rs BBox1Ls BBox.
+ }
+(* swapping in second sequent of principal rule *) 
+*{
+inversion_clear weak; subst;
+acacD' ; subst;
+  try (  acacDe; subst; rem_nil;
+  (cont_setup_apply_constr BBox;
+   use_acm2s_cont' acm rs BBox1Ls BBox) ||
+  (cont_setup_apply_constr2 BBox;
+   use_acm2s_cont' acm rs BBox1Ls BBox) ||
+  (cont_setup_apply_constr3 BBox;
+   use_acm2s_cont' acm rs BBox1Ls BBox)).
+(* 4 subgoals, cases of where swapping occurs in the two parts
+  of context in conclusion (where no principal formula) *)
+
+{ use_acm2s_cont acm rs BBox1Ls. }
+  }
+ }
+ }
+Qed.
+
+Lemma gen_contR_gen_step_b1L_lc: forall V ps concl last_rule rules,
+  last_rule = nslclrule (@b1lrules V) ->
+  gen_contR_gen_step last_rule rules ps concl.
+Proof.  intros until 0.  unfold gen_contR_gen_step.
+intros lreq nsr drs acm rs. clear drs. subst.
+
+inversion nsr as [? ? ? sppc mnsp nsc]. clear nsr.
+unfold nslclext in nsc.
+rewrite can_gen_contR_gen_def'.  intros until 0. intros weak pp ss.
+unfold nslclext in pp. subst.
+
+acacD' ; subst ; rewrite -> ?app_nil_r in *. (* 3 subgoals, the various locs
+  where the exchange might be relative to where the rule is active *)
+
+-{ inversion sppc ; subst ; [> 
+  use_acm_sw_sep_cont acm rs weak WBox1Ls |
+  use_acm_sw_sep_cont acm rs weak BBox1Ls ]. }
+-{ nsgen_sw_cont rs sppc c (Γ, Δ', d) acm inps0 weak. }
+
+-{ inversion sppc ; subst ; clear sppc. (* 2 subgoals *)
++{ acacDe ; subst ; simpl ; rewrite ?app_nil_r. (* 2 subgoals *)
+*{ use_acm_sw_sep_cont acm rs weak WBox1Ls. }
+*{ use_acm_sw_sep_cont acm rs weak WBox1Ls. }
+}
++{ acacDe ; subst ; simpl ; rewrite ?app_nil_r. (* 2 subgoals *)
+*{ use_acm_sw_sep_cont acm rs weak BBox1Ls. }
+*{ use_acm_sw_sep_cont acm rs weak BBox1Ls. }
+}
+}  
+Qed.
+
+(* ------------------------ *)
+(* CONTRACTION FOR B2LRULES *)
+(* ------------------------ *)
+
+Lemma gen_contL_gen_step_b2L_lc: forall V ps concl last_rule rules,
+  last_rule = nslclrule (@b2lrules V) ->
+  gen_contL_gen_step last_rule rules ps concl.
+Proof.  intros until 0.  unfold gen_contL_gen_step.
+intros lreq nsr drs acm rs. (* no clear drs. *) subst.
+
+inversion nsr as [? ? ? sppc mnsp nsc]. clear nsr.
+unfold nslclext in nsc.
+rewrite can_gen_contL_gen_def'.  intros until 0. intros weak pp ss.
+unfold nslclext in pp. subst.
+
+acacD' ; subst ; rewrite -> ?app_nil_r in *. (* 3 subgoals, the various locs
+  where the exchange might be relative to where the rule is active *)
+
+(* weak in the first of the two sequents affected by the rule *)
+-{ inversion sppc ; subst ; clear sppc. (* 2 subgoals *)
++{ inversion_clear weak; subst;
+   acacD' ; subst ; simpl ; rewrite ?app_nil_r; (* 4 subgoals *)
+       acacDe; subst; rem_nil;
+      try (cont_setup_apply_constr4 WBox;
+           use_acm2s_cont' acm rs WBox2Ls WBox);
+      try (cont_setup_apply_constr5 WBox;
+           use_acm2s_cont' acm rs WBox2Ls WBox);
+      try (cont_setup_apply_constr6 WBox;
+           use_acm2s_cont' acm rs WBox2Ls WBox);
+      use_acm2s_cont' acm rs WBox2Ls WBox.
+ }
++{ inversion_clear weak; subst;
+   acacD' ; subst ; simpl ; rewrite ?app_nil_r; (* 4 subgoals *)
+   acacDe; subst; rem_nil;
+      try (cont_setup_apply_constr4 BBox;
+           use_acm2s_cont' acm rs BBox2Ls BBox);
+      try (cont_setup_apply_constr5 BBox;
+           use_acm2s_cont' acm rs BBox2Ls BBox);
+      try (cont_setup_apply_constr6 BBox;
+           use_acm2s_cont' acm rs BBox2Ls BBox);
+      use_acm2s_cont' acm rs BBox2Ls WBox.
+}
+ }
+(* case of exchange in sequent to the left of where rule applied *)
+-{ nsgen_sw_cont rs sppc c (Γ', Δ, d) acm inps0 weak. }
+
+(* here, swap in either of the two sequents affected by the rule *)
+-{ inversion sppc ; subst ; clear sppc. (* 2 subgoals *)
+
+(* WBox *)
+   +{ acacDe ; subst ; simpl ; rewrite ?app_nil_r. (* 2 subgoals *)
++{ inversion_clear weak; subst;
+   acacD' ; subst ; simpl ; rewrite ?app_nil_r; (* 4 subgoals *)
+       acacDe; subst; rem_nil;
+      try (cont_setup_apply_constr4 WBox;
+           use_acm2s_cont' acm rs WBox2Ls WBox);
+      try (cont_setup_apply_constr5 WBox;
+           use_acm2s_cont' acm rs WBox2Ls WBox);
+      try (cont_setup_apply_constr6 WBox;
+           use_acm2s_cont' acm rs WBox2Ls WBox);
+      use_acm2s_cont' acm rs WBox2Ls WBox.
+ }
+
++{ inversion_clear weak; subst;
+   acacD' ; subst ; simpl ; rewrite ?app_nil_r; (* 4 subgoals *)
+   acacDe; subst; rem_nil;
+   try  (list_assoc_r_single; no_use_acm_cont rs drs WBox2Ls);
+   try (   list_assoc_r_single; cont_setup_apply_constr7 WBox;
+           no_use_acm_cont rs drs WBox2Ls).
+ }
+    }
+
+(* BBox *)
+   +{ acacDe ; subst ; simpl ; rewrite ?app_nil_r. (* 2 subgoals *)
++{ inversion_clear weak; subst;
+   acacD' ; subst ; simpl ; rewrite ?app_nil_r; (* 4 subgoals *)
+       acacDe; subst; rem_nil;
+      try (cont_setup_apply_constr4 BBox;
+           use_acm2s_cont' acm rs BBox2Ls BBox);
+      try (cont_setup_apply_constr5 BBox;
+           use_acm2s_cont' acm rs BBox2Ls BBox);
+      try (cont_setup_apply_constr6 BBox;
+           use_acm2s_cont' acm rs BBox2Ls BBox);
+      use_acm2s_cont' acm rs BBox2Ls BBox.
+ }
+ 
++{ inversion_clear weak; subst;
+   acacD' ; subst ; simpl ; rewrite ?app_nil_r; (* 4 subgoals *)
+   acacDe; subst; rem_nil;
+   try  (list_assoc_r_single; no_use_acm_cont rs drs BBox2Ls);
+   try (   list_assoc_r_single; cont_setup_apply_constr7 BBox;
+           no_use_acm_cont rs drs BBox2Ls).
+ }
+    }
+ }
+Qed.
+
+Lemma gen_contR_gen_step_b2L_lc: forall V ps concl last_rule rules,
+  last_rule = nslclrule (@b2lrules V) ->
+  gen_contR_gen_step last_rule rules ps concl.
+Proof.  intros until 0.  unfold gen_contR_gen_step.
+intros lreq nsr drs acm rs. (* no clear drs! *) subst.
+
+inversion nsr as [? ? ? sppc mnsp nsc]. clear nsr.
+unfold nslclext in nsc.
+rewrite can_gen_contR_gen_def'.  intros until 0. intros weak pp ss.
+unfold nslclext in pp. subst.
+
+acacD' ; subst ; rewrite -> ?app_nil_r in *. (* 3 subgoals, the various locs
+  where the exchange might be relative to where the rule is active *)
+
+-{ inversion sppc ; subst ; 
+  [> use_acm_sw_sep_cont acm rs weak WBox2Ls |
+     use_acm_sw_sep_cont acm rs weak BBox2Ls ]. }
+-{ nsgen_sw_cont rs sppc c (Γ, Δ', d) acm inps0 weak. }
+
+-{ inversion sppc ; subst ; clear sppc. (* 2 subgoals *)
++{ acacDe ; subst ; simpl ; rewrite ?app_nil_r. (* 2 subgoals *)
+*{ use_acm_sw_sep_cont acm rs weak WBox2Ls. }
+*{ use_drs rs drs WBox2Ls. }
+}
++{ acacDe ; subst ; simpl ; rewrite ?app_nil_r. (* 2 subgoals *)
+*{ use_acm_sw_sep_cont acm rs weak BBox2Ls. }
+*{ use_drs rs drs BBox2Ls. }
+}
+}  
+Qed.
+
+
+(* ------------------------ *)
+(* CONTRACTION FOR B1RRULES *)
+(* ------------------------ *)
+
+Lemma gen_contL_gen_step_b1R_lc: forall V ps concl last_rule rules,
+  last_rule = nslclrule (@b1rrules V) ->
+  gen_contL_gen_step last_rule rules ps concl.
+Proof.  intros until 0.  unfold gen_contL_gen_step.
+intros lreq nsr drs acm rs. clear drs. subst.
+
+inversion nsr as [? ? ? sppc mnsp nsc]. clear nsr.
+unfold nslclext in nsc.
+rewrite can_gen_contL_gen_def'.  intros until 0. intros swap pp ss.
+unfold nslclext in pp. subst.
+
+acacD' ; subst ; rewrite -> ?app_nil_r in *. (* 3 subgoals, the various locs
+  where the exchange might be relative to where the rule is active *)
+
+-{ inversion sppc ; subst ; clear sppc. (* 2 subgoals *)
+(* swapping in antecedent of first sequent in rule skeleton *)
+   + use_acm_2_cont acm rs swap WBox1Rs.
+   + use_acm_2_cont acm rs swap BBox1Rs.
+ }
+(* case of exchange in sequent to the left of where rule applied,
+  no need to expand sppc *) 
+- contL2 rs sppc acm swap.
+
+-{ inversion sppc ; subst ; clear sppc. (* 2 subgoals *)
+  +{ acacDe ; subst ; simpl ; rewrite ?app_nil_r. (* 2 subgoals *)
+(* swapping in antecedent of first sequent in rule skeleton *)
+* use_acm_2_cont acm rs swap WBox1Rs.
+(* swapping in antecedent of second sequent in rule skeleton *)
+*  use_acm_2_snd_cont acm rs swap WBox1Rs.
+
+}
++{ acacDe ; subst ; simpl ; rewrite ?app_nil_r. (* 2 subgoals *)
+(* swapping in antecedent of first sequent in rule skeleton *)
+* use_acm_2_cont acm rs swap BBox1Rs.
+(* swapping in antecedent of second sequent in rule skeleton *)
+* use_acm_2_snd_cont acm rs swap BBox1Rs.
+ }
+ } 
+Qed.
+
+Lemma gen_contR_gen_step_b1R_lc: forall V ps concl last_rule rules,
+(forall (V : Set) ns
+  (D : derrec rules (fun _ => False) ns),
+      can_gen_swapR rules ns) ->
+  last_rule = nslclrule (@b1rrules V) ->
+  gen_contR_gen_step last_rule rules ps concl.
+Proof.
+  intros until 0. intros Hexch. unfold gen_contR_gen_step.
+  intros lreq nsr drs acm rs. clear drs. subst.
+  inversion nsr as [? ? ? sppc mnsp nsc]. clear nsr.
+  unfold nslclext in nsc.
+  rewrite can_gen_contR_gen_def'.  intros until 0. intros swap pp ss.
+  unfold nslclext in pp. subst.
+  acacD' ; subst ; rem_nil. (* 3 subgoals, the various locs
+  where the exchange might be relative to where the rule is active *)
+
+  -{ inversion sppc ; subst ; clear sppc. (* 2 subgoals, WBox and BBox *)
+     +{ process swap; ltsolve_full acm A rs WBox1Rs a Hexch. }
+     +{ process swap; ltsolve_full acm A rs BBox1Rs a Hexch. }
+   }     
+  -{ contL2 rs sppc acm swap. }
+  -{ inversion sppc ; subst ; clear sppc. (* 2 subgoals, WBox and BBox *)
+     +{ acacDe ; subst ; simpl ; rem_nil. (* 2 subgoals *)
+        (* swap in first sequent in rule skeleton *)
+        *{ process swap ; ltsolve_full acm A rs WBox1Rs a Hexch. }   
+        *{ process swap ; check_nil_cons_contr; 
+           ltsolve_full23 acm A rs WBox WBox1Rs a G. }
+      }
+      
+     +{ acacDe ; subst ; simpl ; rem_nil. (* 2 subgoals *)
+        (* swap in first sequent in rule skeleton *)
+        *{ process swap; ltsolve_full acm A rs BBox1Rs a Hexch. }   
+        *{ process swap; check_nil_cons_contr; 
+           ltsolve_full23 acm A rs BBox BBox1Rs a G. }
+      }
+   }
+Qed.
+
+
+(* ------------------ *)
+(* CONTRACTION FOR EW *)
+(* ------------------ *)
+
+Lemma gen_contR_gen_step_EW_lc: forall V ps concl last_rule rules,
+  last_rule = nslclrule (@EW_rule V) ->
+  gen_contR_gen_step last_rule rules ps concl.
+Proof.  intros until 0.  unfold gen_contR_gen_step.
+intros lreq nsr drs acm rs. subst. (* keep drs in this case *)
+
+inversion nsr as [? ? ? sppc mnsp nsc]. clear nsr.
+unfold nslclext in nsc.
+rewrite can_gen_contR_gen_def'.  intros until 0. intros swap pp ss.
+unfold nslclext in pp. subst.
+
+acacDe ; subst ; rewrite -> ?app_nil_r in *. 
+
+- inversion sppc ; subst ; clear sppc.
+
++ derIrs rs.
+* apply NSlclctxt.  apply EW.
+* apply drs.
+
+- contL2 rs sppc acm swap.
+
+- inversion sppc ; subst ; clear sppc.
+acacDe ; subst ; rewrite -> ?app_nil_r in *.
+derIrs rs.
++ apply NSlclctxt.  apply EW.
++ apply drs.
+Qed.
+
+Lemma gen_contL_gen_step_EW_lc: forall V ps concl last_rule rules,
+  last_rule = nslclrule (@EW_rule V) ->
+  gen_contL_gen_step last_rule rules ps concl.
+Proof.  intros until 0.  unfold gen_contL_gen_step.
+intros lreq nsr drs acm rs. subst. (* keep drs in this case *)
+
+inversion nsr as [? ? ? sppc mnsp nsc]. clear nsr.
+unfold nslclext in nsc.
+rewrite can_gen_contL_gen_def'.  intros until 0. intros swap pp ss.
+unfold nslclext in pp. subst.
+
+acacDe ; subst ; rewrite -> ?app_nil_r in *. 
+
+- inversion sppc ; subst ; clear sppc.
+
++ derIrs rs.
+* apply NSlclctxt.  apply EW.
+* apply drs.
+
+- contL2 rs sppc acm swap.
+
+- inversion sppc ; subst ; clear sppc.
+acacDe ; subst ; rewrite -> ?app_nil_r in *.
+derIrs rs.
++ apply NSlclctxt.  apply EW.
++ apply drs.
+Qed.
+
+
+(* ----------------------------------------- *)
+(* FULL LEFT AND RIGHT CONTRACTION FOR LNSKT *)
+(* ----------------------------------------- *)
+
+Lemma LNSKt_contR_gen: forall (V : Set) ns
+  (D : derrec (@LNSKt_rules V) (fun _ => False) ns),
+      can_gen_contR_gen (@LNSKt_rules V) ns.
+Proof.
+  intros. eapply derrec_all_ind in D.
+  exact D. tauto.
+  intros. inversion H ; subst ;
+          [> pose gen_contR_gen_step_b2R_lc as g
+  | pose gen_contR_gen_step_b1R_lc as g; egx_app g LNSKt_exchR
+  | pose gen_contR_gen_step_b2L_lc as g
+  | pose gen_contR_gen_step_b1L_lc as g
+  | pose gen_contR_gen_step_EW_lc as g
+  | pose gen_contR_gen_step_pr_lc as g ;  egx_app g LNSKt_exchR ]; 
+        unfold gen_contR_gen_step in g; try egx g;
+          clear g ; unfold rsub ; intros ; [> 
+  apply b2r | apply b1r | apply b2l | apply b1l | apply nEW | apply prop ] ;
+  assumption.
+Qed.
+
+Lemma LNSKt_contL_gen: forall (V : Set) ns
+  (D : derrec (@LNSKt_rules V) (fun _ => False) ns),
+      can_gen_contL_gen (@LNSKt_rules V) ns.
+Proof.
+  intros.  eapply derrec_all_ind in D.
+  exact D. tauto.
+  intros. inversion H ; subst ;
+          [> pose gen_contL_gen_step_b2R_lc as g
+  | pose gen_contL_gen_step_b1R_lc as g
+  | pose gen_contL_gen_step_b2L_lc as g
+  | pose gen_contL_gen_step_b1L_lc as g
+  | pose gen_contL_gen_step_EW_lc as g
+  | pose gen_contL_gen_step_pr_lc as g ; egx_app g LNSKt_exchL ]; 
+  unfold gen_contL_gen_step in g; try egx g;
+  clear g ; unfold rsub ; intros;
+  [> apply b2r | apply b1r | apply b2l | apply b1l | apply nEW | apply prop ] ;
+  assumption.
+Qed.
